Defined type ListND for NFAs, updated all NFA operations and proofs, proved the pumping lemma for NFAs

Automata/NFA.lean
@@ -1,35 +1,39 @@
 import Mathlib.Tactic
 import Mathlib.Data.List.Basic
 import Automata.DFA
+import Mathlib.Data.List.Defs
 import Mathlib.Data.FinEnum
 
 open Computability
 
+-- A type for Lists with no duplicates, for synthesizing [Fintype ListND] state from [Fintype state]
+abbrev ListND (α : Type) := {l : List α // l.Nodup}
+
 structure NFA (α state : Type) :=
-  (transition : α → state → List state)
-  (start : List state)
+  (transition : α → state → ListND state)
+  (start : ListND state)
   (output : state → Bool)
 
-def NFA.transList (nfa : NFA α state) (a : α) (qs : List state) [BEq state] : List state :=
-  (qs.bind fun q => nfa.transition a q)
+def NFA.transList (nfa : NFA α state) (a : α) (qs : ListND state) [DecidableEq state] : ListND state :=
+  ⟨(qs.val.bind fun q => nfa.transition a q).dedup, (by apply List.nodup_dedup)⟩
 
-def NFA.evalFrom (nfa : NFA α state) (s : List α) (qs : List state) [BEq state] : Bool :=
+def NFA.evalFrom (nfa : NFA α state) (s : List α) (qs : ListND state) [DecidableEq state] : Bool :=
   match s with
-    | [] => qs.any nfa.output
+    | [] => qs.val.any nfa.output
     | a::as => NFA.evalFrom nfa as (NFA.transList nfa a qs)
 
-def NFA.eval (nfa : NFA α state) (s : List α) [BEq state] : Bool :=
+def NFA.eval (nfa : NFA α state) (s : List α) [DecidableEq state] : Bool :=
   NFA.evalFrom nfa s nfa.start
 
-def NFA.toDFA (nfa : NFA α state) [BEq state] : DFA α (List state) where
+def NFA.toDFA (nfa : NFA α state) [DecidableEq state] : DFA α (ListND state) where
   transition := fun a qs => NFA.transList nfa a qs
   start := nfa.start
-  output := fun qs => qs.any nfa.output
+  output := fun qs => qs.val.any nfa.output
 
-theorem NFA.toDFA_transition (nfa : NFA α state) (a : α) (qs : List state) [BEq state]:
+theorem NFA.toDFA_transition (nfa : NFA α state) (a : α) (qs : ListND state) [DecidableEq state]:
   (nfa.toDFA).transition a qs = NFA.transList nfa a qs := by rfl
 
-theorem NFA.toDFA_evalFrom (nfa : NFA α state) (x : List α) (qs: List state) [BEq state]:
+theorem NFA.toDFA_evalFrom (nfa : NFA α state) (x : List α) (qs: ListND state) [DecidableEq state]:
   (nfa.toDFA).evalFrom x qs = nfa.evalFrom x qs := by
   induction x generalizing qs
   case nil =>
@@ -38,14 +42,22 @@ theorem NFA.toDFA_evalFrom (nfa : NFA α state) (x : List α) (qs: List state) [
     simp only [NFA.evalFrom, DFAO.evalFrom, NFA.toDFA_transition]
     exact ih (nfa.transList y qs)
 
-theorem NFA.toDFA_eval (nfa : NFA α state) (s : List α) [BEq state]
+theorem NFA.toDFA_eval (nfa : NFA α state) (s : List α) [DecidableEq state]
   : (nfa.toDFA).eval s = nfa.eval s := NFA.toDFA_evalFrom nfa s nfa.start
 
-/- TODO
-theorem NFA.pumping_lemma_evalFrom [Fintype state] [BEq state] {nfa : NFA α state} {x : List α} {qs : List state}(hx : nfa.evalFrom x qs)(hlen : Fintype.card state ≤ x.length) :
-    ∃ a b c, x = a ++ b ++ c ∧ a.length + b.length ≤ Fintype.card state ∧ b ≠ []
+
+theorem NFA.pumping_lemma_evalFrom [Fintype state] [DecidableEq state] {nfa : NFA α state} {x : List α} {qs : ListND state}(hx : nfa.evalFrom x qs)(hlen : Fintype.card (ListND state) ≤ x.length) :
+    ∃ a b c, x = a ++ b ++ c ∧ a.length + b.length ≤ Fintype.card (ListND state) ∧ b ≠ []
       ∧ ∀ y ∈ ({a} * {b}∗ * {c} : Language α), nfa.evalFrom y qs := by
   rw [← toDFA_evalFrom] at hx
-  exact nfa.toDFA.pumping_lemma_evalFrom hx hlen
-  done
--/
+  obtain ⟨a, b, c, hxabc, hablen, hne, hy⟩ := nfa.toDFA.pumping_lemma_evalFrom hx hlen
+  use a, b, c
+  constructor
+  . exact hxabc
+  constructor
+  . exact hablen
+  constructor
+  . exact hne
+  intro y h
+  specialize hy y h
+  rwa [← toDFA_evalFrom nfa y qs]
